zoo_std/random_round: Rewrite.

theories/zoo_std/random_round.v
@@ -16,7 +16,7 @@ From zoo_std Require Import
 From zoo Require Import
   options.
 
-Implicit Types i n : nat.
+Implicit Types i n cnt : nat.
 Implicit Types prevs nexts : list nat.
 Implicit Types l : location.
 Implicit Types t rand : val.
@@ -33,6 +33,20 @@ Section zoo_G.
     l.[index] ↦ #(length nexts) ∗
     random_state_model rand ∗
     array_model arr (DfracOwn 1) (#@{nat} <$> nexts ++ reverse prevs).
+  #[local] Instance : CustomIpatFormat "model" :=
+    "(
+      %l &
+      %rand &
+      %arr &
+      %nexts &
+      -> &
+      %Hpermutation &
+      Hl_random &
+      Hl_array &
+      Hl_index &
+      Hrand &
+      Harr
+    )".
 
   Lemma random_round_create_spec sz :
     (0 ≤ sz)%Z →
@@ -46,7 +60,9 @@ Section zoo_G.
     }}}.
   Proof.
     iIntros "%Hsz %Φ _ HΦ".
+
     wp_rec.
+
     pose (Ψ := λ i vs, (
       ⌜vs = #@{nat} <$> seq 0 i⌝
     )%I : iProp Σ).
@@ -55,10 +71,13 @@ Section zoo_G.
       wp_pures.
       iPureIntro. rewrite seq_S fmap_snoc //.
     }
+
     wp_apply (random_state_create_spec with "[//]") as (rand) "Hrand".
     wp_block l as "(Hl_random & Hl_array & Hl_index & _)".
+
     iApply "HΦ".
-    iExists l, rand, arr, (seq 0 ₊sz). rewrite right_id length_seq. iSteps.
+    iFrameSteps. iExists (seq 0 ₊sz).
+    rewrite app_nil_r length_seq. iSteps.
   Qed.
 
   Lemma random_round_reset_spec t sz prevs :
@@ -71,10 +90,13 @@ Section zoo_G.
       random_round_model t sz []
     }}}.
   Proof.
-    iIntros "%Φ (%l & %rand & %arr & %nexts & -> & %Hpermutation & Hl_random & Hl_array & Hl_index & Hrand & Harr) HΦ".
+    iIntros "%Φ (:model) HΦ".
+
     wp_rec. wp_load.
     wp_apply (array_size_spec with "Harr") as "Harr".
-    iSteps. iExists (nexts ++ reverse prevs). rewrite !right_id. iSteps. simpl_length.
+
+    iSteps. iExists (nexts ++ reverse prevs).
+    rewrite app_nil_r. iSteps. simpl_length.
   Qed.
 
   Lemma random_round_next_spec t sz prevs :
@@ -83,60 +105,73 @@ Section zoo_G.
       random_round_model t sz prevs
     }}}
       random_round_next t
-    {{{ i,
-      RET #i;
-      ⌜i < sz ∧ i ∉ prevs⌝ ∗
-      random_round_model t sz (prevs ++ [i])
+    {{{ n,
+      RET #n;
+      ⌜n < sz⌝ ∗
+      ⌜n ∉ prevs⌝ ∗
+      random_round_model t sz (prevs ++ [n])
     }}}.
   Proof.
-    iIntros "%Hprevs %Φ (%l & %rand & %arr & %nexts & -> & %Hpermutation & Hl_random & Hl_array & Hl_index & Hrand & Harr) HΦ".
+    iIntros "%Hprevs %Φ (:model) HΦ".
     pose proof Hpermutation as Hlength%Permutation_length.
     simpl_length in Hlength.
+
     wp_rec. do 3 wp_load.
-    set i := length nexts.
     wp_smart_apply (random_state_int_spec with "Hrand") as (j) "(%Hj & Hrand)"; first lia.
+
     Z_to_nat j.
+    set i := length nexts - 1.
+
     destruct (lookup_lt_is_Some_2 nexts j) as (prev & Hnexts_lookup_j); first lia.
     wp_smart_apply (array_unsafe_get_spec with "Harr") as "Harr".
-    { naive_solver. }
+    { lia. }
     { rewrite list_lookup_fmap. erewrite lookup_app_l_Some => //. }
     { lia. }
-    destruct (lookup_lt_is_Some_2 nexts (i - 1)) as (next & Hnexts_lookup_i); first lia.
+
+    destruct (lookup_lt_is_Some_2 nexts i) as (next & Hnexts_lookup_i); first lia.
     wp_smart_apply (array_unsafe_get_spec with "Harr") as "Harr".
     { lia. }
     { rewrite list_lookup_fmap. erewrite lookup_app_l_Some => //. }
     { lia. }
+
     wp_smart_apply (array_unsafe_set_spec with "Harr") as "Harr".
     { simpl_length. lia. }
     wp_smart_apply (array_unsafe_set_spec with "Harr") as "Harr".
     { simpl_length. lia. }
     wp_store. wp_pures.
-    iApply "HΦ". iSplitR.
-    - iPureIntro. split.
-      + assert (prev ∈ seq 0 sz) as ?%elem_of_seq; last naive_solver.
-        rewrite -Hpermutation elem_of_app elem_of_list_lookup. naive_solver.
-      + pose proof (NoDup_seq 0 sz) as Hnodup.
-        rewrite -Hpermutation NoDup_app in Hnodup.
-        setoid_rewrite elem_of_reverse in Hnodup.
-        setoid_rewrite elem_of_list_lookup at 1 in Hnodup.
-        naive_solver.
-    - rewrite Nat2Z.id -!list_fmap_insert.
-      assert (₊(i - 1) = i - 1) as -> by lia.
-      assert (<[j := next]> (take (i - 1) nexts) ++ [prev] = <[i - 1 := prev]> (<[j := next]> nexts)) as Heq.
-      { destruct_decide (j = i - 1) as -> | H.
-        - rewrite list_insert_ge. { simpl_length. lia. }
-          rewrite list_insert_insert insert_take_drop; first lia.
-          rewrite skipn_all2 //; first lia.
-        - rewrite list_insert_commute // (insert_take_drop nexts); first lia.
-          rewrite skipn_all2; first lia.
-          rewrite -insert_app_l // length_take; first lia.
-      }
-      iSteps. iExists (<[j := next]> (take (i - 1) nexts)). iSteps.
-      + iPureIntro.
-        rewrite -Hpermutation reverse_snoc (assoc _ _ [_]) Heq Permutation_swap' //.
-      + simpl_length. iSteps.
-      + rewrite reverse_snoc (assoc _ _ [_]) Heq insert_app_l; first lia.
-        rewrite insert_app_l // length_insert; first lia.
+
+    iApply "HΦ".
+    iSplitR.
+    { iPureIntro.
+      assert (prev ∈ seq 0 sz) as ?%elem_of_seq; last naive_solver.
+      rewrite -Hpermutation elem_of_app elem_of_list_lookup.
+      naive_solver.
+    }
+    iSplitR.
+    { iPureIntro.
+      pose proof (NoDup_seq 0 sz) as Hnodup.
+      rewrite -Hpermutation NoDup_app in Hnodup.
+      setoid_rewrite elem_of_reverse in Hnodup.
+      setoid_rewrite elem_of_list_lookup at 1 in Hnodup.
+      naive_solver.
+    }
+    rewrite Nat2Z.id -!list_fmap_insert.
+    assert (₊(length nexts - 1) = i) as -> by lia.
+    assert (<[j := next]> (take i nexts) ++ [prev] = <[i := prev]> (<[j := next]> nexts)) as Heq.
+    { destruct_decide (j = i) as -> | H.
+      - rewrite list_insert_ge. { simpl_length. lia. }
+        rewrite list_insert_insert insert_take_drop; first lia.
+        rewrite skipn_all2 //; first lia.
+      - rewrite list_insert_commute // (insert_take_drop nexts); first lia.
+        rewrite skipn_all2; first lia.
+        rewrite -insert_app_l // length_take; first lia.
+    }
+    iSteps. iExists (<[j := next]> (take i nexts)). iSteps.
+    + iPureIntro.
+      rewrite -Hpermutation reverse_snoc (assoc _ _ [_]) Heq Permutation_swap' //.
+    + simpl_length. iSteps.
+    + rewrite reverse_snoc (assoc _ _ [_]) Heq insert_app_l; first lia.
+      rewrite insert_app_l // length_insert; first lia.
   Qed.
 End zoo_G.
 
@@ -148,10 +183,16 @@ From zoo_std Require
 Section zoo_G.
   Context `{zoo_G : !ZooG Σ}.
 
-  Definition random_round_model' t sz n : iProp Σ :=
+  Definition random_round_model' t sz cnt : iProp Σ :=
     ∃ prevs,
-    ⌜(n + length prevs)%nat = sz⌝ ∗
+    ⌜(cnt + length prevs)%nat = sz⌝ ∗
     random_round_model t sz prevs.
+  #[local] Instance : CustomIpatFormat "model'" :=
+    "(
+      %prevs &
+      %H &
+      Ht
+    )".
 
   Lemma random_round_create_spec' sz :
     (0 ≤ sz)%Z →
@@ -165,13 +206,14 @@ Section zoo_G.
     }}}.
   Proof.
     iIntros "%Hsz %Φ _ HΦ".
+
     wp_apply (random_round_create_spec with "[//]") as (t) "Ht"; first done.
-    iSteps. iExists []. iSteps.
+    iStepFrameSteps.
   Qed.
 
-  Lemma random_round_reset_spec' t sz n :
+  Lemma random_round_reset_spec' t sz cnt :
     {{{
-      random_round_model' t sz n
+      random_round_model' t sz cnt
     }}}
       random_round_reset t
     {{{
@@ -179,24 +221,26 @@ Section zoo_G.
       random_round_model' t sz sz
     }}}.
   Proof.
-    iIntros "%Φ (%prevs & %H & Ht) HΦ".
+    iIntros "%Φ (:model') HΦ".
+
     wp_apply (random_round_reset_spec with "Ht") as "Ht".
-    iSteps. iExists []. iSteps.
+    iStepFrameSteps.
   Qed.
 
-  Lemma random_round_next_spec' t sz n :
-    0 < n →
+  Lemma random_round_next_spec' t sz cnt :
+    0 < cnt →
     {{{
-      random_round_model' t sz n
+      random_round_model' t sz cnt
     }}}
       random_round_next t
-    {{{ i,
-      RET #i;
-      ⌜i < sz⌝ ∗
-      random_round_model' t sz (n - 1)
+    {{{ n,
+      RET #n;
+      ⌜n < sz⌝ ∗
+      random_round_model' t sz (cnt - 1)
     }}}.
   Proof.
-    iIntros "%Hn %Φ (%prevs & %H & Ht) HΦ".
+    iIntros "%Hcnt %Φ (:model') HΦ".
+
     wp_apply (random_round_next_spec with "Ht") as (i) "(%Hi & Ht)"; first lia.
     iSteps. iExists (prevs ++ [i]). simpl_length. iSteps.
   Qed.
